\documentclass[9pt]{beamer}
\usepackage{xeCJK}

\usetheme{Berkeley}
\usefonttheme[onlymath]{serif}
\usepackage[utf8]{inputenc}
\usepackage[T1]{fontenc}
\usepackage{amsmath}
\usepackage{amsfonts}
\usepackage{amssymb}
\usepackage{multicol}

\title{哈哈}
\subtitle{快速傅里叶变换}
\author{丁尧尧}
\institute{上海交通大学}
\date{\today}
\usetheme{CambridgeUS}

\begin{document}
	\begin{frame}
		\begin{align*}
			A(x) = \sum_{i=0}^na_ix^i = a_nx^n+a_{n-1}x^{n-1}+\cdots+a_1x+a_0 \\ 
			B(x) = \sum_{i=0}^nb_ix^i = b_nx^n+b_{n-1}x^{n-1}+\cdots+b_1x+b_0
		\end{align*}
		\begin{align*}
			A(\omega_n^k) = \sum_{i=0}^{n-1}a_i\omega^{ki} , k = 0, 1, \cdots, n - 1
		\end{align*}
		
		\begin{eqnarray*} 
			A(\omega_n^k) &=& \sum_{i=0}^{n-1}a_i\omega_n^{ki} \\
			 &=&\sum_{i=0}^{\frac{n}{2}-1}a_{2i}\omega_n^{2ki}+\omega_n^k\sum_{i=0}^{\frac{n}{2}-1}a_{2i+1}\omega_n^{2ki} \\ 
		\end{eqnarray*}
		\begin{align*}
		\omega_n^2=\left(e^{\frac{2\pi i}{n}}\right)^2=e^{\frac{2\pi i}{n/2}}=\omega_{\frac{n}{2}}
		\end{align*}
		
	\end{frame}	
	\begin{frame}
		设$k < \frac{n}{2}$:
		\begin{align*}
			A(\omega_n^k) = \sum_{i=0}^{\frac{n}{2}-1}a_{2i}\omega_{\frac{n}{2}}^{ki}+\omega_n^{k}\sum_{i=0}^{\frac{n}{2}-1}a_{2i+1}\omega_{\frac{n}{2}}^{ki}
		\end{align*}
		\begin{eqnarray*} 
			A(\omega_n^{k+\frac{n}{2}}) &=& \sum_{i=0}^{\frac{n}{2}-1}a_{2i}\omega_{\frac{n}{2}}^{ki}+\omega_n^{k+\frac{n}{2}}\sum_{i=0}^{\frac{n}{2}-1}a_{2i+1}\omega_{\frac{n}{2}}^{ki} \\ &=&\sum_{i=0}^{\frac{n}{2}-1}a_{2i}\omega_{\frac{n}{2}}^{ki}-\omega_n^k\sum_{i=0}^{\frac{n}{2}-1}a_{2i+1}\omega_{\frac{n}{2}}^{ki} 
		\end{eqnarray*}
		\begin{align*}
		T(n) = 2T(\frac{n}{2})+\mathcal O(n) = \mathcal O(n\log n)
		\end{align*}
		
	\end{frame}
	\begin{frame}
		\begin{equation} \label{IDFT-equation} \begin{bmatrix} (\omega_n^0)^0 & (\omega_n^0)^1 & \cdots & (\omega_n^0)^{n-1} \\ (\omega_n^1)^0 & (\omega_n^1)^1 & \cdots & (\omega_n^1)^{n-1} \\ \vdots & \vdots & \ddots & \vdots \\ (\omega_n^{n-1})^0 & (\omega_n^{n-1})^1 & \cdots & (\omega_n^{n-1})^{n-1} \end{bmatrix} \begin{bmatrix} a_0 \\ a_1 \\ \vdots \\ a_{n-1} \end{bmatrix} = \begin{bmatrix} A(\omega_n^0) \\ A(\omega_n^1) \\ \vdots \\ A(\omega_n^{n-1}) \end{bmatrix} \end{equation}
		系数矩阵的逆矩阵：
		\begin{equation*} \mathbf D = \begin{bmatrix} (\omega_n^{-0})^0 & (\omega_n^{-0})^1 & \cdots & (\omega_n^{-0})^{n-1} \\ (\omega_n^{-1})^0 & (\omega_n^{-1})^1 & \cdots & (\omega_n^{-1})^{n-1} \\ \vdots & \vdots & \ddots & \vdots \\ (\omega_n^{-(n-1)})^0 & (\omega_n^{-(n-1)})^1 & \cdots & (\omega_n^{-(n-1)})^{n-1} \end{bmatrix} \end{equation*}
	\end{frame}
\end{document} 

